theorems/iN.lean
@@ -2,6 +2,8 @@ import theorems.iN.SimpSets
 import theorems.iN.iN_def
 import theorems.iN.iN_llvm
 import theorems.iN.iN_rewrite
+import theorems.iN.iN_lattice
+import theorems.iN.iN_bitvec
 import theorems.iN.tactics.iN_tactic_blast
 import theorems.iN.tactics.iN_tactic_rewrite
 import theorems.iN.tactics.iN_tactic_opt
