theorems/iN/iN_bitvec.lean
@@ -1,0 +1,48 @@
+import theorems.iN.iN_def
+import theorems.iN.iN_llvm
+
+/-- `poison_unroll x y z => a b c`
+
+Performs `cases x; cases y; cases z`, solves every `poison` branch with
+`simp [iN_unwrap_inst]`, and in the unique `bitvec` branch introduces the
+payloads named `a b c`. -/
+syntax "poison_unroll" (ppSpace colGt ident)* " =>" (ppSpace colGt ident)* : tactic
+macro_rules
+| `(tactic| poison_unroll $xs:ident* => $ys:ident*) =>
+  `(tactic|
+    ($[cases $xs:ident with
+      | bitvec $ys:ident => ?_
+      | poison => simp [simp_iN]];*);
+
+      simp at * /- simp hypotheses with bitvec -/
+    )
+
+theorem BitVec.saddOverflow_comm {n} {a b : BitVec n}
+    : a.saddOverflow b = b.saddOverflow a := by
+
+  grind [BitVec.saddOverflow]
+
+theorem BitVec.uaddOverflow_comm {n} {a b : BitVec n}
+    : a.uaddOverflow b = b.uaddOverflow a := by
+
+  grind [BitVec.uaddOverflow]
+
+
+theorem saddOverflow_iff_or {n} (x y : BitVec n)
+    : x.saddOverflow y
+      ↔ x.toInt + y.toInt ≥ 2 ^ (n - 1) ∨ x.toInt + y.toInt < - 2 ^ (n - 1) := by
+
+  unfold BitVec.saddOverflow
+  rw [← Bool.decide_or]
+  rw [decide_eq_true_eq]
+
+
+theorem addNsw_saddOverflow_bitvec {n} {a b : BitVec n} (h : a.saddOverflow b)
+    : (bitvec a) +nsw (bitvec b) = poison := by
+
+  simp [simp_iN, h]
+
+theorem addNsw_not_saddOverflow_bitvec_eq_add {n} {a b : BitVec n} (h : ¬a.saddOverflow b)
+    : (bitvec a) +nsw (bitvec b) = bitvec (a + b) := by
+
+  simp [simp_iN, h]
