theorems/iN/iN_lattice.lean
@@ -1,0 +1,44 @@
+import theorems.iN.iN_def
+
+structure Interval (bits : Nat) : Type where
+  lo : BitVec bits := BitVec.intMin bits
+  hi : BitVec bits := BitVec.intMax bits
+
+def Interval.mem {n} (int : Interval n) : iN n → Prop
+  | poison => True
+  | bitvec a => int.lo.toInt ≤ a.toInt ∧ a.toInt ≤ int.hi.toInt
+
+/- instance instMembe {n} : Membership (iN n) (Interval n) where
+  mem := Interval.mem -/
+
+/- TODO instance actually unwrapping to the thing fix  -/
+notation:50 a:50 " ∈ " b:50 => Interval.mem b a
+
+syntax:100 "i[" term ",∞]" : term
+syntax:100 "i[-∞," term "]" : term
+syntax:100 "i[" term "," term "]" : term
+
+macro_rules
+  | `(i[$a:term,∞]) => `({ lo := $a : Interval _})
+  | `(i[-∞,$b:term]) => `({ hi := $b : Interval _})
+  | `(i[$a:term,$b:term]) => `({ lo := $a, hi := $b : Interval _})
+
+@[simp]
+theorem Interval.bitvec_mem_lo_iff_ineq {n} (a : BitVec n) (lo : BitVec n)
+    : bitvec a ∈ { lo := lo : Interval n} ↔ lo.toInt ≤ a.toInt := by
+
+  simp [Interval.mem, BitVec.toInt_le]
+
+@[simp]
+theorem Interval.bitvec_mem_hi_iff_ineq {n} (a : BitVec n) (hi : BitVec n)
+    : bitvec a ∈ { hi := hi : Interval n} ↔ a.toInt ≤ hi.toInt := by
+
+  by_cases h : (0 < n)
+  case pos =>
+    simp [Interval.mem, BitVec.toInt_intMin_of_pos h, BitVec.le_toInt]
+
+  case neg =>
+
+    have h' : n = 0 := by omega
+    subst h'
+    grind [Interval.mem]
